coq/coq/Translation.v
@@ -103,12 +103,6 @@ Definition styp2ttyp_raw (A: typ) : ttyp :=
 
 Notation "[[ A ]]" := (styp2ttyp_raw A) (at level 5, A at next level).
 
-Lemma translate_eqv : forall A B,
-    || A || = || B || -> eqIndTypTarget [[ A ]] [[ B ]].
-
-
-#[local] Hint Constructors wf_typ : core.
-
 
 Lemma translate_to_record_types : forall A,
     rec_typ |[ A ]|.
@@ -116,15 +110,95 @@ Proof with eauto using rcd_typ_concat_simpl.
   introv. induction A; simpl...
 Qed.
 
-Lemma lookup_concat_simpl_none : forall i A B,
-    Tlookup l |[A]| = Some  -> rec_typ A ->
-    Tlookup i (ttyp_concat_simpl A B) = Tlookup i B.
-Proof.
-  introv LK HR. gen i B.
-  induction A; intros; simpl; try solve_by_invert; eauto.
-  - inverts* HR. inverts LK. case_if.
-    forwards* Heq: IHA2.
+(* Typ-TopAbs requires no ord *)
+Lemma ttyp_trans_ord_top : forall A,
+    toplike A -> |[A]| = ttyp_top.
+Admitted.
+
+
+Lemma eqindextype_complete : forall A B,
+    || A || = || B || -> eqIndTyp A B.
+Proof with eauto.
+  introv H.
+  (* -> direction ? *)
+Admitted.
+
+
+Lemma eqindextype_sound : forall A B,
+    eqIndTyp A B -> || A || = || B ||.
+Proof with eauto.
+  introv H. induction* H.
+    + rewrite* IHeqIndTyp1.
+    + simpl.
+Admitted.
+
+Lemma eqIndTypTarget_concat_comm : forall A B,
+    rec_typ A -> rec_typ B ->
+    eqIndTypTarget (ttyp_concat_simpl A B) (ttyp_concat_simpl B A).
+Proof with eauto.
+  introv HA HB. gen B.
+  induction* HA; intros; induction* HB; simpl...
+  - simpl in IHHB.
+    applys TEI_trans. applys TEI_rcd. applys TEI_refl. applys* IHHA.
+    applys TEI_trans. simpl. apply TEI_comm.
+    applys TEI_rcd. applys TEI_refl. applys* IHHB.
 Qed.
+
+Lemma ttyp_concat_simpl_assoc : forall A B C,
+    rec_typ A -> rec_typ B -> rec_typ C ->
+    (ttyp_concat_simpl (ttyp_concat_simpl A B) C) = ttyp_concat_simpl A (ttyp_concat_simpl B C).
+Proof with simpl in *; eauto.
+  introv HRA HRB HRC.
+  induction HRA...
+  rewrite IHHRA...
+Qed.
+
+
+Lemma eqIndTypTarget_ttyp_concat_simpl : forall A1 A2 B1 B2,
+    eqIndTypTarget A1 A2 -> eqIndTypTarget B1 B2 ->
+    eqIndTypTarget (ttyp_concat_simpl A1 B1) (ttyp_concat_simpl A2 B2).
+Proof with eauto using translate_to_record_types.
+  introv HEA HEB. gen B1 B2.
+  induction HEA; intros.
+  - induction* At. simpl...
+  - applys TEI_trans.
+    + forwards*: IHHEA1. + forwards*: IHHEA2.
+  - applys* TEI_symm.
+  - simpl...
+  - simpl...
+  - simpl...
+Qed.
+
+Lemma translate_eqv : forall A B,
+    eqIndTyp A B -> eqIndTypTarget |[ A ]| |[ B ]|.
+Proof with eauto using translate_to_record_types.
+  introv HE. lets HE': HE. induction* HE'.
+  - forwards Heq: eqindextype_sound HE.
+    unfolds styp2ttyp. rewrite Heq. simpl...
+  - forwards Heq: eqindextype_sound HE.
+    unfolds styp2ttyp. rewrite Heq. simpl...
+  - simpl. forwards*: IHHE'.
+    applys* eqIndTypTarget_ttyp_concat_simpl.
+  - simpl. forwards Heq: eqindextype_sound HE.
+    applys eqIndTypTarget_concat_comm...
+  - simpl. rewrite* ttyp_concat_simpl_assoc...
+  - simpl. rewrite* ttyp_trans_ord_top.
+  - simpl. forwards*: IHHE'. (* dedup or not dedup *) admit.
+Admitted.
+
+#[local] Hint Constructors wf_typ : core.
+
+
+
+(* Lemma lookup_concat_simpl_none : forall i A B, *)
+(*     Tlookup l |[A]| = Some  -> rec_typ A -> *)
+(*                     Tlookup i (ttyp_concat_simpl A B) = Tlookup i B. *)
+(* Proof. *)
+(*   introv LK HR. gen i B. *)
+(*   induction A; intros; simpl; try solve_by_invert; eauto. *)
+(*   - inverts* HR. inverts LK. case_if. *)
+(*     forwards* Heq: IHA2. *)
+(* Qed. *)
 
 
 Lemma ttyp_trans_wf : forall A,
@@ -139,38 +213,88 @@ Proof with intuition eauto using rcd_typ_concat_simpl.
       * forwards* Heq: lookup_concat_simpl H.
         rewrite H in Heq...
       * forwards* Heq: lookup_concat_simpl_none |[ A2 ]| H...
-        rewrite H in Heq...
         applys* WF_Rcd...
 Admitted.
 
-(* Typ-TopAbs requires no ord *)
-Lemma ttyp_trans_ord_top : forall A,
-    toplike A -> |[A]| = ttyp_top.
-Admitted.
 
-Lemma ttyp_trans_ord_ntop : forall A,
-    ord A -> ~ toplike A -> exists B, |[A]| = (ttyp_rcd (||A||) B ttyp_top) /\ wf_typ B.
-Admitted.
+(* Lemma ttyp_trans_ord_ntop : forall A, *)
+(*     ord A -> ~ toplike A -> exists B, |[A]| = (ttyp_rcd (||A||) B ttyp_top) /\ wf_typ B. *)
+(* Admitted. *)
 
-Lemma ttyp_trans_base :
-    |[typ_base]| = ttyp_rcd (||typ_base||) ttyp_base ttyp_top.
-Admitted.
+(* Lemma ttyp_trans_base : *)
+(* |[typ_base]| = ttyp_rcd (||typ_base||) ttyp_base ttyp_top. *)
+(* Admitted. *)
 
-Lemma ttyp_trans_ord_ntop_arrow : forall A A',
-    (* ord A -> ~ toplike A -> *) (* S-arrow requires no precondition *)
-    |[(typ_arrow A' A)]| = ttyp_rcd (||typ_arrow A' A||) (ttyp_arrow |[A']| |[A]|) ttyp_top.
-Admitted.
+(* Lemma ttyp_trans_ord_ntop_arrow : forall A', A *)
+(* (* ord A -> ~ toplike A -> *) (* S-arrow requires no precondition *) *)
+(* |[(typ_arrow A' A)]| = ttyp_rcd (||typ_arrow A' A||) (ttyp_arrow |[A']| |[A]|) ttyp_top. *)
+(* Admitted. *)
 
-Lemma ttyp_trans_rcd : forall l A,
-    (* ord A -> ~ toplike A -> *) (* S-arrow requires no precondition *)
-    |[(typ_rcd l A)]| = ttyp_rcd (||(typ_rcd l A)||) |[A]| ttyp_top.
-Admitted.
+(* Lemma ttyp_trans_rcd : forall l A, *)
+(* (* ord A -> ~ toplike A -> *) (* S-arrow requires no precondition *) *)
+(* |[(typ_rcd l A)]| = ttyp_rcd (||(typ_rcd l A)||) |[A]| ttyp_top. *)
+(* Admitted. *)
 
-Lemma ttyp_trans_and : forall A B C,
-    concat_typ |[ A ]| |[ B ]| C -> |[ (typ_and A B) ]| = C.
-Admitted.
+(* Lemma ttyp_trans_and : forall A B C, *)
+(*     concat_typ |[ A ]| |[ B ]| C -> |[ (typ_and A B) ]| = C. *)
+(* Admitted. *)
 
 (* Properties about type translation *)
 Lemma concat_source_intersection : forall A B,
     concat_typ |[ A ]| |[ B ]| |[ (typ_and A B) ]|.
+Admitted.
+
+
+
+Lemma eqIndTypTarget_wf_typ : forall A B,
+    eqIndTypTarget A B -> wf_typ A -> wf_typ B.
+Proof.
+Admitted.
+
+Lemma eqIndTypTarget_rec_typ : forall A B,
+    eqIndTypTarget A B -> rec_typ A -> rec_typ B.
+Proof.
+Admitted.
+
+Lemma eqIndTypTarget_lookup_none : forall A B l,
+    eqIndTypTarget A B -> Tlookup l A = None -> Tlookup l B = None.
+Proof.
+Admitted.
+
+Lemma eqIndTypTarget_lookup_some : forall A B l C,
+    eqIndTypTarget A B -> Tlookup l A = Some C ->
+    exists C', eqIndTypTarget C C' /\ Tlookup l B = Some C'.
+Proof.
+Admitted.
+
+Lemma eqIndTypTarget_concat_typ : forall A B C A' B',
+    concat_typ A B C -> eqIndTypTarget A A' -> eqIndTypTarget B B' ->
+    exists C', concat_typ A' B' C' /\ eqIndTypTarget C C'.
+Proof.
+Admitted.
+
+Lemma eqIndTypTarget_arrow_inv : forall A B C,
+    eqIndTypTarget (ttyp_arrow A B) C -> exists C1 C2, C = ttyp_arrow C1 C2.
+Proof with eauto.
+  introv HE. inductions HE...
+  - forwards* (?&?&?): IHHE1. subst*.
+    forwards* (?&?&?): IHHE2.
+Admitted.
+
+Lemma eqIndTypTarget_rcd_inv : forall l A B C1 C2,
+    eqIndTypTarget (ttyp_rcd l A B) (ttyp_rcd l C1 C2) -> A = C1.
+Proof with eauto.
+  introv HE. inductions HE...
+Admitted.
+
+Lemma eqIndTypTarget_arrow_inv_1 : forall A B C1 C2,
+    eqIndTypTarget (ttyp_arrow A B) (ttyp_arrow C1 C2) -> eqIndTypTarget A C1.
+Proof with eauto.
+  introv HE. inductions HE...
+Admitted.
+
+Lemma eqIndTypTarget_arrow_inv_2 : forall A B C1 C2,
+    eqIndTypTarget (ttyp_arrow A B) (ttyp_arrow C1 C2) -> eqIndTypTarget B C2.
+Proof with eauto.
+  introv HE. inductions HE...
 Admitted.
